Config.v
@@ -1,0 +1,160 @@
+From CHSTLC Require Import Terms.
+From Coq Require Import Lists.List.
+Import ListNotations.
+From Coq Require Import Lia.
+
+Definition buffer := list tm.
+
+Definition channels := list buffer.
+
+Inductive config : Type :=
+| Config : channels -> list tm -> config
+.
+
+Fixpoint update {A} (n : nat) (a : A) (l : list A) : (list A) :=
+match l with
+| [] => l
+| h :: t => match n with
+          | 0 => a :: t
+          | S n' => h :: (update n' a t)
+          end
+end.
+
+Fixpoint give_chs (n : nat) (v : tm) (chs : channels) :=
+match chs with
+| [] => []
+| h :: t => match n with
+          | O => (h ++ [v]) :: t
+          | S n' => h :: (give_chs n' v t)
+          end
+end.
+
+Inductive cfg_step : config -> config -> Prop :=
+| cs_give : forall E n T v result1 result2 chs thrds,
+    value v -> fillCtx E (tm_give (tm_ch n T) v) result1 ->
+    fillCtx E (tm_unit) result2 ->
+    n < length chs -> cfg_step (Config chs (result1 :: thrds)) (Config (give_chs n v chs) (result2 :: thrds))
+| cs_take : forall E n T result1 result2 chs thrds v t,
+    fillCtx E (tm_take (tm_ch n T)) result1 ->
+    fillCtx E v result2 ->
+    n < length chs -> nth_error chs n = Some (v :: t) ->
+    cfg_step (Config chs (result1 :: thrds)) (Config (update n t chs) (result2 :: thrds))
+| cs_fork : forall E t result1 result2 chs thrds,
+    fillCtx E (tm_fork t) result1 ->
+    fillCtx E (tm_unit) result2 ->
+    cfg_step (Config chs (result1 :: thrds)) (Config chs ([t; result2] ++ thrds))
+| cs_mkch : forall E T result1 result2 chs thrds,
+    fillCtx E (tm_mkch T) result1 ->
+    fillCtx E (tm_ch (length thrds) T) result2 ->
+    cfg_step (Config chs (result1 :: thrds)) (Config (chs ++ [[]]) (result2 :: thrds))
+| cs_term : forall E t1 t2 result1 result2 chs thrds,
+    fillCtx E t1 result1 ->
+    fillCtx E t2 result2 ->
+    step t1 t2 ->
+    cfg_step (Config chs (result1 :: thrds)) (Config chs (result2 :: thrds))
+| cs_sub : forall E t t' result result' chs chs' thrds, fillCtx E t result ->
+                                             fillCtx E t' result' ->
+                                             cfg_step (Config chs (t :: thrds)) (Config chs' (t' :: thrds)) ->
+                                             cfg_step (Config chs (result :: thrds)) (Config chs' (result' :: thrds))
+| cs_pop : forall v chs thrds,
+    value v -> cfg_step (Config chs (v :: thrds)) (Config chs thrds)
+.
+
+Global Hint Constructors cfg_step : core.
+
+Lemma nth_error_some_length : forall A n l (v : A), Some v = nth_error l n -> n < length l.
+Proof.
+  intros. apply nth_error_Some. intros contr. rewrite <- H in contr. inversion contr.
+Qed.
+
+Lemma subterm_swap : forall E t t' result, fillCtx E t result -> exists result', fillCtx E t' result'.
+Proof.
+  induction E; intros; eauto.
+  - inversion H; subst. eapply IHE in H4. destruct H4. eauto.
+  - inversion H; subst. eapply IHE in H5. destruct H5. eauto.
+  - inversion H; subst. eapply IHE in H5. destruct H5. eauto.
+  - inversion H; subst. eapply IHE in H1. destruct H1. eauto.
+  - inversion H; subst. eapply IHE in H4. destruct H4. eauto.
+  - inversion H; subst. eapply IHE in H5. destruct H5. eauto.
+  - inversion H; subst. eapply IHE in H1. destruct H1. eauto.
+Qed.
+
+Fixpoint channels_bounded (t : tm) (chs : channels) :=
+match t with
+| tm_var x => True
+| tm_abs x T t => channels_bounded t chs
+| tm_unit => True
+| tm_app t1 t2 => channels_bounded t1 chs /\ channels_bounded t2 chs
+| tm_let x t1 t2 => channels_bounded t1 chs /\ channels_bounded t2 chs
+| tm_fork t => channels_bounded t chs
+| tm_give t1 t2 => channels_bounded t1 chs /\ channels_bounded t2 chs
+| tm_take t => channels_bounded t chs
+| tm_mkch T => True
+| tm_ch n T => n < length chs
+end.
+
+Lemma subterm_bounded : forall E t result chs, fillCtx E t result -> channels_bounded result chs ->
+                                          channels_bounded t chs.
+Proof.
+  induction E; intros; inversion H; subst; try destruct H0; eauto.
+Qed.
+
+Theorem config_progress : forall c,
+match c with
+| Config chs thrds => match thrds with
+                     | [] => True
+                     | h :: t => forall T, empty ⊢ h ∈ T -> channels_bounded h chs ->
+                                    (value h) \/ (exists h' chs', h' <> [] -> cfg_step c (Config chs' (h' ++ t))) \/
+                                      (exists E n T, fillCtx E (tm_take (tm_ch n T)) h ->
+                                                nth_error chs n = Some [])
+                     end
+end.
+  intros [chs thrds].
+  destruct thrds; auto. intros.
+  assert (H' := H).
+  apply progress in H. destruct H as [ | []].
+  - auto.
+  - destruct H. right. left. exists [x], chs. simpl. eauto.
+  - destruct H as [E H]. destruct H as [|[|[]]].
+    + destruct H. right. left. assert (H'' := H). eapply subterm_swap in H. destruct H. exists [x0]. simpl. eauto.
+    + destruct H as (c & H & H1). assert (H'' := H).
+      eapply subterm_type in H; eauto. destruct H. inversion H; subst.
+      apply canonical_channel in H4; auto. destruct H4; subst. right. remember (nth_error chs x0).
+      destruct o.
+      * destruct b.
+        {
+          right. exists E, x0, x. intros. auto.
+        }
+        {
+          left. assert (H''' := H''). apply subterm_swap with (t' := t0) in H'''. destruct H'''.
+          exists [x1]. simpl. eexists. intros. eapply cs_take. eapply H''. eapply H2. apply nth_error_some_length in Heqo. auto.
+          symmetry in Heqo. eapply Heqo.
+        }
+      * eapply subterm_bounded in H''; eauto. simpl in H''. symmetry in Heqo. apply nth_error_None in Heqo.
+        lia.
+    + destruct H as (c & v & H & H1 & H2). assert (H'' := H).
+      eapply subterm_type in H; eauto. destruct H. inversion H; subst. apply canonical_channel in H6; auto.
+      destruct H6; subst. right. left. assert (H''' := H''). apply subterm_swap with (t' := tm_unit) in H''.
+      destruct H''. exists [x0]. simpl. eexists. intros.  eapply cs_give; eauto. eapply subterm_bounded in H'''; eauto.
+      simpl in H'''. destruct H'''. auto.
+    (* + destruct H as (f & H & H1). right. left. do 2 eexists. eapply cs_sub. eapply H. *)
+      (* apply subterm_swap with (t' := tm_unit) in H. destruct H. eapply H. *)
+    + destruct H as (f & H & H1). right. left. assert (H'' := H). apply subterm_swap with (t' := tm_unit) in H.
+      destruct H. exists [f; x], chs. intros. eauto.
+Qed.
+
+(* Theorem cfg_preservation : forall c, *)
+(*     match c with *)
+(*     | Config chs thrds => match thrds with *)
+(*                          | [] => True *)
+(*                          | h :: t => forall h' T chs' f, empty ⊢ h ∈ T -> *)
+(*                                                      cfg_step (Config chs (h::t)) (Config chs' (f ++ [h'] ++ t)) -> *)
+(*                                                      empty ⊢ h' ∈ T *)
+(*                          end *)
+(*     end. *)
+(* Proof. *)
+(*   intros [chs thrds]. *)
+(*   destruct thrds as [|h t]; trivial. *)
+(*   intros. generalize dependent T. remember (f ++ [h'] ++ t). destruct l. *)
+(*   - destruct f; inversion Heql. *)
+(*   - induction H0; intros. *)
